Prove tulip RA except initialization

src/program_proof/tulip/res_network.v
@@ -1,3 +1,4 @@
+From iris.algebra Require Import gmap_view.
 From Perennial.program_proof Require Import grove_prelude.
 From Perennial.program_proof.tulip Require Import base.
 
@@ -6,26 +7,60 @@ Section res.
   (* TODO: remove this once we have real defintions for resources. *)
   Implicit Type (γ : tulip_names).
 
-  Definition own_terminals γ (gid : u64) (ts : gset chan) : iProp Σ.
-  Admitted.
+  Definition is_terminal γ (gid : u64) (t : chan) : iProp Σ :=
+    own γ.(group_trmlm) {[ gid := gmap_view_frag t DfracDiscarded tt ]}.
 
-  Definition is_terminal γ (gid : u64) (t : chan) : iProp Σ.
-  Admitted.
+  Definition own_terminals_auth γ (gid : u64) (ts : gset chan) : iProp Σ :=
+    own γ.(group_trmlm) {[ gid := gmap_view_auth (DfracOwn 1) (gset_to_gmap tt ts) ]}.
+
+  Definition own_terminals γ (gid : u64) (ts : gset chan) : iProp Σ :=
+    own_terminals_auth γ gid ts ∗ ([∗ set] t ∈ ts, is_terminal γ gid t).
 
   #[global]
   Instance is_terminal_persistent γ gid t :
     Persistent (is_terminal γ gid t).
-  Admitted.
+  Proof. apply _. Defined.
 
   Lemma terminal_update {γ gid ts} t :
     own_terminals γ gid ts ==∗
     own_terminals γ gid ({[t]} ∪ ts) ∗ is_terminal γ gid t.
-  Admitted.
+  Proof.
+    iIntros "[Hauth #Hfrags]".
+    destruct (decide (t ∈ ts)) as [Hin | Hnotin].
+    { replace (_ ∪ _) with ts by set_solver.
+      iDestruct (big_sepS_elem_of with "Hfrags") as "#Hfrag".
+      { apply Hin. }
+      by iFrame "∗ #".
+    }
+    set ts' := _ ∪ _.
+    iAssert (own_terminals_auth γ gid ts' ∗
+             is_terminal γ gid t)%I
+      with "[> Hauth]" as "[Hauth #Hfrag]".
+    { iRevert "Hauth".
+      rewrite -own_op.
+      iApply own_update.
+      rewrite singleton_op.
+      apply singleton_update.
+      rewrite gset_to_gmap_union_singleton.
+      apply: gmap_view_alloc; last done; last done.
+      by rewrite lookup_gset_to_gmap_None.
+    }
+    iFrame "∗ #".
+    by iApply big_sepS_insert_2.
+  Qed.
 
   Lemma terminal_lookup γ gid ts t :
     is_terminal γ gid t -∗
     own_terminals γ gid ts -∗
     ⌜t ∈ ts⌝.
-  Admitted.
+  Proof.
+    iIntros "#Hfrag [Hauth _]".
+    iDestruct (own_valid_2 with "Hauth Hfrag") as %Hvalid.
+    rewrite singleton_op singleton_valid in Hvalid.
+    apply gmap_view_both_dfrac_valid_discrete_total in Hvalid.
+    destruct Hvalid as (v' & _ & _ & Hlookup & _ & _).
+    apply elem_of_dom_2 in Hlookup.
+    by rewrite dom_gset_to_gmap in Hlookup.
+  Qed.
 
 End res.
